SStructTT/Dynamic/Renaming.lean
@@ -1,3 +1,4 @@
+import SStructTT.Static.Renaming
 import SStructTT.Dynamic.Typed
 
 namespace Dynamic
@@ -25,4 +26,53 @@ where
     AgreeRen ξ Γ Δ Γ' Δ' ->
     AgreeRen (ξ !>> (.+1)) Γ Δ (A :: Γ') (_: Δ')
 
--- lemma AgreeRen.toStatic
+lemma AgreeRen.toStatic {Γ Γ' : Static.Ctx Srt} {Δ Δ' : Dynamic.Ctx Srt} {ξ} :
+    Dynamic.AgreeRen ξ Γ Δ Γ' Δ' -> Static.AgreeRen ξ Γ Γ' := by
+  intro agr
+  induction agr <;> aesop (rule_sets := [rename])
+
+@[aesop safe (rule_sets := [rename])]
+lemma AgreeRen.refl {Γ : Static.Ctx Srt} {Δ : Dynamic.Ctx Srt} :
+    Γ ; Δ ⊢ -> AgreeRen id Γ Δ Γ Δ := by
+  intro wf; induction wf <;> try aesop (rule_sets := [rename])
+  case ex ty _ agr =>
+    have agr := agr.ex ty
+    asimp at agr
+    assumption
+  case im ty _ agr =>
+    have agr := agr.im ty
+    asimp at agr
+    assumption
+
+lemma AgreeRen.none {Γ Γ' : Static.Ctx Srt} {Δ Δ' : Dynamic.Ctx Srt} {ξ} :
+    AgreeRen ξ Γ Δ Γ' Δ' -> Δ.Forall (. = none) -> Δ'.Forall (. = none) := by
+  intro agr; induction agr <;> aesop
+
+lemma AgreeRen.has {Γ Γ' : Static.Ctx Srt} {Δ Δ' : Dynamic.Ctx Srt} {ξ x s A} :
+    Dynamic.AgreeRen ξ Γ Δ Γ' Δ' ->
+    Has Δ x s A ->
+    Has Δ' (ξ x) s A.[ren ξ] := by
+  intro agr
+  induction agr generalizing x s A
+  case nil =>
+    intro h; cases h
+  case ex A _ _ ξ _ agr ih =>
+    intro h;
+    rcases h with ⟨h⟩
+    have h := agr.none h
+    asimp
+    rw[show A.[ren ξ !> shift 1] = A.[ren ξ].[shift 1] by asimp]
+    constructor; assumption
+  case im B _ _ ξ _ agr ih =>
+    intro h;
+    cases h with | @cons _ A x _ h =>
+    specialize ih h
+    asimp
+    rw[show A.[ren ξ !> shift 1] = A.[ren ξ].[shift 1] by asimp]
+    constructor; assumption
+  case wk ξ _ _ ih =>
+    intro h
+    specialize ih h
+    asimp
+    rw[show A.[ren (ξ !>> (.+1))] = A.[ren ξ].[shift 1] by asimp; rfl]
+    constructor; assumption
